LambdaS5/coq/LjsPrettyRulesSecurity.v
@@ -1,0 +1,158 @@
+Generalizable All Variables.
+Set Implicit Arguments.
+Require Import Utils.
+Require Import LjsShared.
+Require Import LjsSyntax.
+Require Import LjsPrettyInterm.
+Require Import LjsPrettyRules.
+Require Import LjsPrettyRulesIndexed.
+Require Import LjsPrettyRulesIndexedInvert.
+Require Import LjsStore.
+Require Import LjsCommon.
+Require Import LjsValues.
+Require Import LjsOperators.
+Require Import LjsMonads.
+Require Import JsNumber.
+Import List.ListNotations.
+
+Open Scope list_scope.
+
+Implicit Type st : store.
+Implicit Type e : expr.
+Implicit Type v : value.
+Implicit Type s : string.
+Implicit Type n : number.
+Implicit Type i : id.
+Implicit Type o : out.
+Implicit Type c : ctx.
+Implicit Type ptr : object_ptr.
+Implicit Type obj : object.
+Implicit Type attrs : attributes.
+
+Inductive attributes_security_ok : attributes -> attributes -> Prop := 
+| attributes_security_ok_accessor : forall acc,
+    attributes_security_ok (attributes_accessor_of acc) (attributes_accessor_of acc)
+| attributes_security_ok_data_unwritable : forall data,
+    !attributes_data_writable data ->
+    attributes_security_ok (attributes_data_of data) (attributes_data_of data)
+| attributes_security_ok_data_writable : forall data data',
+    attributes_data_writable data ->
+    attributes_data_enumerable data = attributes_data_enumerable data' ->
+    attributes_data_configurable data = attributes_data_configurable data' ->
+    attributes_security_ok (attributes_data_of data) (attributes_data_of data')
+.
+
+Record object_security_ok obj obj' : Prop := {
+    object_security_ok_class :
+        object_class obj = object_class obj';
+    object_security_ok_code :
+        object_code obj = object_code obj';
+    object_security_ok_proto : 
+        !object_extensible obj -> object_proto obj = object_proto obj';
+    object_security_ok_extensible : 
+        !object_extensible obj -> !object_extensible obj';
+    object_security_ok_properties : 
+        !object_extensible obj -> forall s, index (object_properties obj') s -> index (object_properties obj) s;
+    object_security_ok_attributes : forall s attrs,
+        binds (object_properties obj) s attrs -> 
+        !attributes_configurable attrs -> 
+        exists attrs',
+        binds (object_properties obj') s attrs' /\ 
+        !attributes_configurable attrs' /\
+        attributes_security_ok attrs attrs'
+}.
+
+Definition state_security_ok st st' : Prop :=
+    forall ptr obj,
+    binds st ptr obj -> exists obj',
+    binds st' ptr obj' /\
+    object_security_ok obj obj'.
+
+Lemma attributes_security_ok_refl : refl attributes_security_ok.
+Proof.
+    intro attrs.
+    destruct attrs as [()|()].
+    destruct attributes_data_writable.
+    apply attributes_security_ok_data_writable; auto.
+    apply attributes_security_ok_data_unwritable; auto.
+    apply attributes_security_ok_accessor.
+Qed.
+
+Lemma object_security_ok_refl : refl object_security_ok.
+Proof.
+    intro obj.
+    destruct obj.
+    destruct object_attrs.
+    constructor; eauto using attributes_security_ok_refl.
+Qed.
+
+Lemma state_security_ok_refl : refl state_security_ok.
+Proof.
+    intro st. unfolds. eauto using object_security_ok_refl.
+Qed.
+
+Lemma attributes_security_ok_trans : trans attributes_security_ok.
+Proof.
+    introv Hs1 Hs2.
+    inverts Hs1; inverts Hs2.
+    apply attributes_security_ok_accessor.
+    apply attributes_security_ok_data_unwritable; auto.
+    rew_refl in *; tryfalse.
+    apply attributes_security_ok_data_writable; auto.
+    apply attributes_security_ok_data_writable; auto; eapply eq_trans; eauto.
+Qed.
+
+Lemma object_security_ok_trans : trans object_security_ok.
+Proof.
+    introv Hs1 Hs2.
+    inverts Hs1. inverts Hs2.
+    constructor. 
+    eapply eq_trans; eauto.
+    eapply eq_trans; eauto.
+    intro. apply (eq_trans (object_proto y)); eauto. 
+    eauto.
+    eauto.
+    introv Hbinds1 Hc1.
+    specializes object_security_ok_attributes0 Hbinds1 Hc1.
+    destruct object_security_ok_attributes0 as (?attrs&Hbinds2&Hc2&Hok1).
+    specializes object_security_ok_attributes1 Hbinds2 Hc2.
+    destruct object_security_ok_attributes1 as (?attrs&Hbinds3&Hc3&Hok2).
+    jauto_set; eauto. applys attributes_security_ok_trans Hok1 Hok2.
+Qed.
+
+Lemma state_security_ok_trans : trans state_security_ok.
+Proof.
+    introv Hs1 Hs2.
+    unfolds state_security_ok.
+    introv Hbinds1.
+    specializes Hs1 Hbinds1.
+    destruct Hs1 as (?obj&Hbinds2&Hok1).
+    specializes Hs2 Hbinds2.
+    destruct Hs2 as (?obj&Hbinds3&Hok2).
+    jauto_set; eauto. applys object_security_ok_trans Hok1 Hok2.
+Qed.
+
+Local Ltac ljs_inv := 
+    match goal with
+    | H : red_exprh _ _ _ ?e _ |- _=>
+        match e with
+        | expr_basic _ => fail 1
+        | _ => inverts red_exprh H; tryfalse
+        end
+    end.
+
+Lemma red_exprh_state_security_ok : forall k c st st' r e,
+    red_exprh k c st e (out_ter st' r) ->
+    state_security_ok st st'.
+Proof.
+    intro k.
+    induction k;
+    introv Hred. 
+    inverts Hred.
+    destruct e;
+    inverts red_exprh Hred;
+    try apply state_security_ok_refl.
+    skip.
+    repeat ljs_inv. 
+(* TODO *)
+Admitted.
